Add in-progress LL(1) completeness proof, and a motivating example for handling EOF

LL1/ParserTests.v
@@ -6,5 +6,29 @@ Open Scope string_scope.
 Example test1 :
   parse g311ParseTable (NT "S") g311Sentence1 100 =
   (Some g311ParseTree1, nil).
-Proof. simpl. reflexivity. Defined.
+Proof. simpl. reflexivity. Qed.
+
+(* We should be able to parse the empty input string, but
+   there's no way to do this at the moment because the parser
+   requires a lookahead token. I'm going to try to fix this
+   by modifying the parser so that when it encounters an empty 
+   input string, it checks whether the next grammar symbol is
+   a special EOF symbol. *)
+Definition x_y_grammar :=
+  [(NT "x", [NT "y"]);
+     (NT "y", [])].
+
+Definition x_map := SymbolMap.empty (list symbol).
+Definition y_map := SymbolMap.empty (list symbol).
+Definition x_y_parse_table :=
+  SymbolMap.add
+    (NT "x") x_map
+    (SymbolMap.add
+       (NT "y") y_map
+       (SymbolMap.empty (SymbolMap.t (list symbol)))).
+                
+Example x_y_test1 :
+  parse x_y_parse_table (NT "x") nil 100 =
+  (Some (Node "x" Fnil), nil).
+Proof. simpl. Abort.
 
