LL1/CompletenessProof.v
@@ -1,0 +1,118 @@
+Require Import List String.
+Require Import Derivation Grammar Lemmas ParseTable ParseTree LL1.Parser Lib.Tactics.
+
+Conjecture pre_suf_nil : forall A (prefix suffix : list A),
+    (prefix ++ suffix)%list = suffix ->
+    prefix = nil.
+
+Lemma tree_forest_fuel :
+  forall g tbl gamma input fuel suffix subtrees ntName,
+    isParseTableFor tbl g ->
+    In (NT ntName, gamma) g ->
+    parseForest tbl gamma input fuel = (Some subtrees, suffix) ->
+    parse tbl (NT ntName) input (S fuel) = (Some (Node ntName subtrees), suffix).
+Proof.
+  intros.
+  destruct fuel as [| fuel].
+  - inv H1.
+  - destruct gamma as [| sym gamma'].
+    + (* gamma is nil *)
+      simpl in H1. (* now we know that parseForest
+                      produces an empty list of subtrees *)
+      inv H1.
+      destruct suffix as [| token suffix'].
+      * simpl.
+        (* The problem is that there's no lookahead token,
+           which isn't a problem for parseForest, but IS a
+           problem for parse *)
+Abort.
+      
+Conjecture forest_fuel_tree_fuel :
+  forall tbl gamma input fuel suffix subtrees ntName,
+    parseForest tbl gamma input fuel =
+    (Some subtrees, suffix) ->
+    parse tbl (NT ntName) input (S fuel) =
+    (Some (Node ntName subtrees), suffix).
+
+Conjecture hd_fuel_tl_fuel_forest_fuel :
+  forall tbl hdRoot tlRoots xs ys zs tr f fuel,
+    parse tbl hdRoot (app (app xs ys) zs) fuel =
+    (Some tr, app ys zs) ->
+    parseForest tbl tlRoots (app ys zs) fuel = (Some f, zs) ->
+    parseForest tbl (hdRoot :: tlRoots) (app (app xs ys) zs) fuel = (Some (Fcons tr f), zs).
+
+Theorem parse_complete :
+  forall (g   : grammar)
+         (tbl : parse_table),
+    isParseTableFor tbl g ->
+    forall (tr     : tree)
+           (input  : list string)
+           (sym    : symbol)
+           (prefix suffix : list string),
+      input = (prefix ++ suffix)%list ->
+      (@derivesTree g) sym prefix tr ->
+      exists (fuel : nat),
+        parse tbl sym input fuel = (Some tr, suffix).
+Proof.
+  intros g tbl Htbl tr.
+  induction tr as [ s
+                  | s f IHparseForest
+                  |
+                  | tr IHparse f IHparseForest ]
+      using tree_mutual_ind with
+      (P := fun tr =>
+              forall input sym prefix suffix,
+                input = (prefix ++ suffix)%list ->
+                (@derivesTree g) sym prefix tr ->
+                exists (fuel : nat),
+                  parse tbl sym input fuel = (Some tr, suffix))
+      (P0 := fun subtrees =>
+               forall input gamma prefix suffix,
+                 input = (prefix ++ suffix)%list ->
+                 (@derivesForest g) gamma prefix subtrees ->
+                 exists fuel,
+                   parseForest tbl gamma input fuel = (Some subtrees, suffix)).
+  
+  - intros input sym prefix suffix Hinput HderivesTree.
+    inv HderivesTree.
+    exists 1. simpl.
+    destruct (Utils.beqSym (T s) (T s)) eqn:Hbeq.
+    + reflexivity.
+    + unfold Utils.beqSym in Hbeq.
+      destruct (SymbolMapFacts.eq_dec) in Hbeq.
+      * inv Hbeq.
+      * exfalso. apply n. reflexivity.
+        
+  - intros input sym prefix suffix Hinput HderivesTree.
+    inv HderivesTree.
+    apply IHparseForest with (prefix := prefix)
+                             (suffix := suffix)
+                             (input := app prefix suffix)
+      in H4; clear IHparseForest.
+    + destruct H4 as [fuel].
+      exists (S fuel).
+      eapply forest_fuel_tree_fuel. eassumption.
+    + reflexivity.
+      
+  - intros input gamma prefix suffix Hinput HderivesForest.
+    inv HderivesForest.
+    exists 1. simpl. reflexivity.
+    
+  - intros input gamma prefix suffix Hinput HderivesForest.
+    inv HderivesForest.
+    apply IHparse with
+        (input := ((prefix0 ++ suffix0)%list ++ suffix)%list)
+        (suffix := (suffix0 ++ suffix)%list) in H3;
+      clear IHparse.
+    + destruct H3 as [hdFuel].
+      apply IHparseForest with
+      (input := (suffix0 ++ suffix)%list)
+          (suffix := suffix) in H4; clear IHparseForest.
+      * destruct H4 as [tlFuel].
+        exists (S (hdFuel + tlFuel)).
+        simpl.
+        (* Here, we can prove a lemma saying that if 
+           hdFuel is enough to produce the left sibling, 
+           then so is (hdFuel + tlFuel), and then do the
+           same thing for tlFuel *)
+Abort.
